

## SOLVING QUADRATIC EQUATIONS

*Your task: complete the problems below. Solutions are given at the end of the document; attempt **and check** all questions before verifying your answers.*

---

1. Solve for  $x$  by factorising each equation.

- (a)  $x^2 - 4x - 19 = 2$ ,
- (b)  $3x^2 + 10x + 4 = x^2 + x$ ,
- (c)  $3x^2 - 6x + 3 = 0$ ,
- (d)  $5x^2 + 89x - 18 = 0$ .

2. Solve for  $x$  by completing the square.

- (a)  $x^2 - 8x + 6 = 0$ ,
- (b)  $x^2 + 10x - 17 = 0$ ,
- (c)  $3x^2 - 21x + 31 = 0$ .

3. Explain how you have checked your answers in questions 1(a-d) and 2(a-c).

4. What is the quadratic formula? And, in your own words, explain where it comes from.

5. Use the quadratic formula to solve 1(b).

**Solutions. 1.** In 1(a-b) remember to first set your right-hand side to zero. Otherwise we factorise as normal,

- (a)  $x^2 - 4x - 21 = 0 \iff (x - 7)(x + 3) = 0$ , so  $x = 7$  or  $x = -3$ ;  
 (b)  $2x^2 + 9x + 4 = 0 \iff (2x + 1)(x + 4) = 0$ , so  $x = -\frac{1}{2}$  or  $x = -4$ ;  
 (c)  $3x^2 - 6x + 3 = 0 \iff 3(x^2 - 2x + 1) = 0 \iff 3(x - 1)^2 = 0$ , so  $x = 1$  only;  
 (d)  $5x^2 + 89x - 18 = 0 \iff (5x - 1)(x + 18) = 0$ , so  $x = \frac{1}{5}$  or  $x = -18$ .

**2.** For (a), if  $x^2 - 8x + 6 = 0$  then

$$\begin{aligned}(x - 4)^2 - (-4)^2 + 6 &= 0 \\(x - 4)^2 - 16 + 6 &= 0 \\(x - 4)^2 &= 10 \\x - 4 &= \pm\sqrt{10}\end{aligned}$$

and therefore  $x = 4 \pm \sqrt{10}$ .

**(b)** If  $x^2 + 10x - 17 = 0$  then

$$\begin{aligned}(x + 5)^2 - (5)^2 - 17 &= 0 \\(x + 5)^2 - 25 - 17 &= 0 \\(x + 5)^2 &= 42 \\x + 5 &= \pm\sqrt{42}\end{aligned}$$

so  $x = -5 \pm \sqrt{42}$ .

**(c)** If  $3x^2 - 21x + 31 = 0$ , we need to factor out the leading coefficient of 3. The constant term +31 does not need to be included. So

$$\begin{aligned}3(x^2 - 7x) + 31 &= 0 \\3\left[\left(x - \frac{7}{2}\right)^2 - \left(-\frac{7}{2}\right)^2\right] + 31 &= 0 \\3\left[\left(x - \frac{7}{2}\right)^2 - \frac{49}{4}\right] + 31 &= 0.\end{aligned}$$

In these types of problem it common to have to deal with fractions. At this step you should think about moving terms to the right hand side,

$$\begin{aligned}3\left(x - \frac{7}{2}\right)^2 - \frac{147}{4} &= -31 \\3\left(x - \frac{7}{2}\right)^2 &= \frac{23}{4} \\ \left(x - \frac{7}{2}\right)^2 &= \frac{23}{12} \\x - \frac{7}{2} &= \pm\sqrt{\frac{23}{12}}\end{aligned}$$

so  $x = \frac{7}{2} \pm \sqrt{\frac{23}{12}}$ . You could simplify the surd if you like. This question is no different to the others in principle; it just had trickier algebra with fractions.

**3.** You can check your solutions for these problems by substituting in your  $x$ -values into the original equation. For example, in 1(b) we found  $x = -4$  or  $x = -\frac{1}{2}$ . We could check  $x = -4$  by calculating  $2x^2 + 9x + 4 = 0$ , i.e.

$$2(-4)^2 + 9(-4) + 4 = 2(16) - 36 + 4 = 32 - 36 + 4 = 0,$$

as it should be.

**4.** For a quadratic  $ax^2 + bx + c$ , the quadratic formula is

$$x = \frac{-b \pm \sqrt{b^2 - 4ac}}{2a}.$$

It is derived by completing the square on the general form of a quadratic above.

**5.** For 1(b), we have  $2x^2 + 9x + 4 = 0$ . So then

$$x = \frac{-9 \pm \sqrt{81 - 4(2)(4)}}{4} = \frac{-9 \pm \sqrt{49}}{4} = \frac{-9 \pm 7}{4}$$

so  $x = \frac{-9+7}{4} = \frac{-2}{4} = -\frac{1}{2}$ , or  $x = \frac{-9-7}{4} = -4$ . These are the same answers as before.